\subsection{Problem 6(2.21)}
\begin{flushleft}
    \textbf{Solution: }
    Let $ S_n = \sum_{k=0}^{n} (-1)^{n-k} $
    \par
    Now,
    % solve using perturbation method
    $$
        \begin{aligned}
            S_{n+1}   & = \sum_{k=0}^{n+1} (-1)^{n+1-k}  \\
            \Rightarrow \sum_{k=0}^{n} (-1)^{n+1-k} + (-1)^{n+1-(n+1)}   & = (-1)^{n+1-0} + \sum_{k=1}^{n+1} (-1)^{n+1-k}                \\
            \Rightarrow \sum_{k=0}^{n} (-1)^{n-k} \cdot (-1)^1 + (-1)^0   & = (-1)^{n+1} + \sum_{1 \leq k+1 \leq n+1}^{} (-1)^{n+1-(k+1)} \\
            \Rightarrow -S_n + 1 & = (-1)^{n+1} + \sum_{0 \leq k \leq n} (-1)^{n-k}              \\
            \Rightarrow  -S_n + 1 & = (-1)^{n+1} + S_n              \\
            \Rightarrow 2S_n & = 1 + (-1)^{n+1} \\
            \Rightarrow S_n & = \frac{1 + (-1)^{n+1}}{2} \\
        \end{aligned}
    $$

    \par

    Again let, $ T_n = \sum_{k=0}^{n} (-1)^k k $
    \par
    Now,
    % solve using perturbation method
    $$
    \begin{aligned}
        T_{n+1} &= \sum_{k=0}^{n+1} (-1)^k k \\
        \Rightarrow T_{n+1} &= (-1)^{n+1-0} \cdot 0 + \sum_{k=1}^{n+1} (-1)^{n+1-k} k \\
        \Rightarrow \sum_{k=0}^{n} (-1)^{n+1-k}k + (-1)^{n+1-(n+1)} \cdot (n+1) &= \sum_{1 \leq k+1 \leq n+1} (-1)^{n+1-(k+1)}(k+1)\\
        \Rightarrow \sum_{k=0}^{n} (-1)^{n-k} \cdot k \cdot (-1)^1 + (n+1) &= \sum_{0 \leq k \leq n} (-1)^{n-k}(k+1)\\
        \Rightarrow -T_n + (n+1) &= \sum_{0 \leq k \leq n} (-1)^{n-k}k + \sum_{0 \leq k \leq n} (-1)^{n-k} \\
        \Rightarrow -T_n + (n+1) &= T_n + S_n \\
        \Rightarrow 2T_n &= (n+1) - S_n \\
        \Rightarrow T_n &= \frac{(n+1) - S_n}{2} \\
                        &= \frac{(n+1) - \frac{1 + (-1)^{n+1}}{2}}{2} \\
                        &= \frac{2(n+1) - (1 + (-1)^{n+1})}{4} \\
                        &= \frac{2n + 2 - 1 - (-1)^{n+1}}{4} \\
                        &= \frac{2n + 1 + (-1)^{n+1}}{4} \\
    \end{aligned}
    $$

\end{flushleft}