\subsection{Problem 4(2.19)}
\textbf{Use a summation factor to solve the recurrence
$$
\begin{aligned}
T_0 & =5 \\
2 T_n & =n T_{n-1}+3 \cdot n !, \quad \text { for } n>0 .
\end{aligned}
$$}
\par

\begin{flushleft}
\textbf{Solution: }
\par
Given recurrence,
$$
\begin{aligned}
T_0 & =5 \\
2 T_n & =n T_{n-1}+3 \cdot n !
\end{aligned}
$$
Comparing with $a_n T_n=b_n T_{n-1}+c_n$, we get
$$
a_n=2, b_n=n \text { and } c_n=3 \cdot n !
$$
So, the summation factor,
$$
\begin{aligned}
s_n & =\frac{a_{n-1} a_{n-2} \cdots a_1}{b_n b_{n-1} \cdots b_2} \\
& =\frac{2 \cdot 2 \cdot \cdots 2}{n(n-1) \cdots 2} \\
& =\frac{2^{n-1}}{n !}
\end{aligned}
$$
Therefore,
$$
\begin{aligned}
T_n & =\frac{1}{s_n a_n}\left(s_1 b_1 T_0 + \sum_{k=1}^n s_k c_k\right) \\
& =\frac{1}{s_n a_n}\left(\frac{2^{1-1}}{1 !} \cdot 1 \cdot 5+\sum_{k=1}^n \frac{2^{k-1}}{k !} \cdot 3 \cdot k !\right) \\
& =\frac{1}{\frac{2^{n-1}}{n !}} \cdot 2\left(\frac{n !}{2^n}\left(5+3 \sum_{k=1}^n 2^{k-1}\right)\right. \\
& =\frac{n !}{2^n}\left(5+3\left(2^n-1\right)\right) \\
& =\frac{n !}{2^n}\left(2+3 \cdot 2^n\right) \\
& =n !\left(2^{1-n}+3\right) \quad
\end{aligned}
$$

\end{flushleft}



