\subsection{Problem 7(2.23)}
\textbf{Evaluate the sum $ \sum_{k=1}^{n} (2k+1)/k(k+1)$ using partial fraction.}
\par

\begin{flushleft}
    \textbf{Solution: }
    \par
    % partial fraction using thumb rule
    Here,
    $$
        \begin{aligned}
            \frac{2k+1}{k(k+1)} & = \frac{2\cdot0 + 1}{k(0+1)} + \frac{2 \cdot (-1) + 1}{(-1)(k+1)} \\
            & = \frac{1}{k} + \frac{1}{k+1} \\
        \end{aligned}
    $$

    Now, 
    $$
    \begin{aligned}
        \sum_{k=1}^{n} \frac{2k+1}{k(k+1)} & =  \sum_{k=1}^{n} \left( \frac{1}{k} + \frac{1}{k+1} \right)  \\
        & = \sum_{k=1}^{n} \frac{1}{k} + \sum_{k=1}^{n} \frac{1}{k+1} \\
        & = H_n + \sum_{1 \leq k \leq n} \frac{1}{k+1} \\
        % replace k with k-1 in r.h.s
        & = H_n + \sum_{1 \leq k-1 \leq n} \frac{1}{(k-1)+1} \\
        % add 1 to each side of the limit of the sum
        & = H_n + \sum_{2 \leq k \leq n+1} \frac{1}{k} \\
        % make harmonic
        & = H_n +  \sum_{1 \leq k \leq n} \frac{1}{k} + \frac{1}{n+1} - \frac{1}{1}\\
        & = H_n + H_n + \frac{1}{n+1} - 1 \\
        & = 2H_n - \frac{n}{n+1} \\
    \end{aligned}
    $$

\end{flushleft}