\subsection{Problem 5}
\textbf{}
\par

\begin{flushleft}
\textbf{Solution: }
\par
Let $ S_n = \sum_{k=0}^{n} kH_k $
\par
Now,
% solve using perturbation method
$$
\begin{aligned}
    S_{n+1} &= \sum_{k=0}^{n+1} kH_k \\
    \Rightarrow S_{n+1} &= 0 \cdot H_0 + \sum_{k=1}^{n+1} kH_k \\
    \Rightarrow S_{n+1} &= \sum_{1 \leq k+1 \leq n+1}^{} (k+1)H_{k+1} \\
    \Rightarrow S_{n+1} &= \sum_{0 \leq k \leq n} (k+1)(H_k + \frac{1}{k+1}) \\
    \Rightarrow S_{n+1} &= \sum_{0 \leq k \leq n} (1 + kH_k + H_k) \\
    \Rightarrow S_{n+1} &= \sum_{0 \leq k \leq n} 1 + \sum_{0 \leq k \leq n} kH_k + \sum_{0 \leq k \leq n} H_k \\
    \Rightarrow S_n + (n+1)H_{n+1} &= (n+1) + S_n + \sum_{0 \leq k \leq n} H_k \\
    % find summation of H_k
    \Rightarrow \sum_{0 \leq k \leq n} H_k &= (n+1) - (n+1)H_{n+1} \\
    & = (n+1)(1-H_{n+1})  
\end{aligned}
$$
\end{flushleft}