\subsection{Problem 3(2.14)}
\textbf{}
\par

\begin{flushleft}
\textbf{Solution: }
\par
$\begin{aligned} 
\sum_{k=1}^n k 2^k & =\sum_{k=1}^n\left(\sum_{j=1}^k 1\right)^k \\
& =\sum_{k=1}^n \sum_{j=1}^k 2^k \\
& =\sum_{1 \leq j \leq k \leq n} 2^k \\
& =\sum_{1 \leq j \leq n} \sum_{j \leq k \leq n} 2^k \\
& =\sum_{1 \leq j \leq n}\left(\sum_{0 \leq k \leq n} 2^k-\sum_{0 \leq k \leq j-1} 2^k\right) \\
& =\sum_{1 \leq j \leq n}\left(2^{n+1} -1 -2^j + 1 \right) \\
& =\sum_{1 \leq j \leq n} 2^{n+1}-\sum_{1 \leq j \leq n} 2^j \\
& =2^{n+1} \sum_{1 \leq j \leq n} 1-\left(\sum_{0 \leq j \leq n} 2^j-1\right) \\
& =n 2^{n+1}-\left(2^{n+1}-1-1\right) \\
& =n 2^{n+1}-\left(2^{n+1}-2\right)
\end{aligned}
$
\end{flushleft}